messing with trans

Constellation/FunRel.lean
@@ -13,47 +13,29 @@ inductive ReflClos {α: Sort u} (R: EndoRel α): EndoRel α where
 inductive TransClos {α: Sort u} (R: EndoRel α): EndoRel α where
   | base x y  :           R x y →
                 TransClos R x y
-  | step x y z: TransClos R x y →
-                          R   y z →
-                TransClos R   y z
-
-theorem tr_rt {α: Sort u}:
-  ∀ (R: EndoRel α) (x y: α),
-    ReflClos (TransClos R) x y
-    ↔
-    TransClos (ReflClos R) x y
-:= by
-  intro R x y
-  constructor
-  . intro h
-    cases h
-    . constructor
-      constructor
-    . next h =>
-      cases h
-      . constructor
-        constructor
-        assumption
-      . constructor
-        constructor
-        assumption
-  . intro h
-    cases h
-    . next h =>
-      cases h
-      . constructor
-      . constructor
-        constructor
-        assumption
-    . next _ _ h =>
-      cases h
-      . constructor
-      . constructor
-        constructor
-        assumption
+  | step x y z:           R x y →
+                TransClos R   y z →
+                TransClos R x   z
 
 notation:max R "⊹" => TransClos R
-notation:max R "⋆" => ReflClos (R⊹)
+notation:max R "⋆" => ReflClos  R⊹
+
+namespace TransClos
+
+  theorem midstep {α: Sort u} {R: EndoRel α} {x y z: α}
+    (h1: R⊹ x y)
+    (h2: R⊹   y z)
+  :      R⊹ x   z
+  := by
+    induction h1
+    . case base a b h =>
+      exact TransClos.step _ _ _ h h2
+    . case step a b c h1 h3 ih =>
+      exact TransClos.step _ _ _ h1 (ih h2)
+
+end TransClos
+
+
 
 namespace List
   def any_Prop: List Prop → Prop :=
